Refactoring

src/common/Curve25519_Operations.ec
@@ -1,24 +1,24 @@
 require import Bool List Int IntDiv CoreMap Real Ring StdOrder.
-require import Zp_25519 Zplimbs Curve25519_Spec.
-import Zp StdOrder.IntOrder Ring.IntID Array4.
+require import Zp_25519 Zplimbs Curve25519_Spec EClib.
+import Zp StdOrder.IntOrder Ring.IntID Array4 EClib.
 
 from Jasmin require import JModel.
 
-
-(* sets msb to 0 *)
-op msb_to_zero (x: Rep4) = let x = x.[3 <- x.[3].[63 <- false]] in x.
+(* sets last bit to 0 *)
+op last_bit_to_zero64 (x: Rep4) : Rep4 = let x = x.[3 <- x.[3].[63 <- false]] in x.
 
 (* returns the first 2 elements of the input triple *)
-op select_double_from_triple (t : ('a * 'a) * ('a * 'a) * 'c) = (t.`1, t.`2).
+op select_double_from_triple (t : ('a * 'a) * ('a * 'a) * 'c) : ('a * 'a) * ('a * 'a) = (t.`1, t.`2).
 
-(* if the third element is true then the first 2 elements are swapped *)
-  (*  - this op returns the first 2 elements in
-  the correct order       *)
-op reconstruct_triple (t : ('a * 'a) * ('a * 'a) * bool) =
+(* if the third element is true then the first 2 elements are swapped
+  - this op returns the first 2 elements in the correct order      *)
+op reconstruct_triple (t : ('a * 'a) * ('a * 'a) * bool) : ('a * 'a) * ('a * 'a)  =
     if t.`3
     then spec_swap_tuple (select_double_from_triple t)
     else select_double_from_triple t.
 
+(* given that t.`3 is false, we can convert from a "list" with two elems
+   to a ""list"" with three elements, whereby the last element is false *)
 lemma eq_reconstruct_select_triple (t : (('a * 'a) * ('a * 'a) * bool)) :
     t.`3 = false =>
     select_double_from_triple t = reconstruct_triple t.
@@ -27,57 +27,52 @@ proof.
     by move => ? /#.
 qed.
 
-(* move elsewhere *)
-lemma foldl_in_eq_r (f1 : 'a1 -> 'b -> 'a1)
-                    (f2 : 'a2 -> 'b -> 'a2)
-                    (s  : 'b list)
-                    (a2 : 'a2)
-                    (r  : 'a2 -> 'a1) :
-    (forall a2 b, b \in s => f1 (r a2) b = r (f2 a2 b)) =>
-                        foldl f1 (r a2) s = r (foldl f2 a2 s).
-proof.
-    move: s a2. elim.
-        by move => a2.
-    move => x l hrec a2 /= hin. rewrite hin.
-    by left.
-    rewrite hrec //; move => ? ? h; rewrite hin.
-        by right.
-    by trivial.
-qed.
 
-(** step1: spec_add_and_double = op_add_and_double : reordered to match implementation **)
-op op_add_and_double (qx : zp) (nqs : (zp * zp) * (zp * zp)) =
-    let x_1 = qx                                      in
-    let (x_2, z_2) = nqs.`1                           in
-    let (x_3, z_3) = nqs.`2                           in
-    let a          = x_2  +  z_2                      in
-    let aa         = a    *  a                        in
-    let b          = x_2  -  z_2                      in
-    let bb         = b    *  b                        in
-    let e          = aa   -  bb                       in
-    let c          = x_3  +  z_3                      in
-    let d          = x_3  -  z_3                      in
-    let da         = d    *  a                        in
-    let cb         = c    *  b                        in
-    let x_3        = (da  +  cb)  *  (da + cb)        in
-    let z_3        = x_1  *  ((da - cb) * (da - cb))  in
-    let x_2        = aa   *  bb                       in
-    let z_2        = e    *  (aa + (inzp 121665 * e)) in
+(* step 1: spec_add_and_double = op_add_and_double : reordered to match
+    implementation *)
+op op_add_and_double (qx : zp, nqs : (zp * zp) * (zp * zp)) : (zp * zp) * (zp * zp)  =
+    let x_1 = qx                                   in
+    let (x_2, z_2) = nqs.`1                        in
+    let (x_3, z_3) = nqs.`2                        in
+    let a          = x_2 + z_2                     in
+    let aa         = a * a                         in
+    let b          = x_2 - z_2                     in
+    let bb         = b *  b                        in
+    let e          = aa - bb                       in
+    let c          = x_3 + z_3                     in
+    let d          = x_3 - z_3                     in
+    let da         = d * a                         in
+    let cb         = c * b                         in
+    let x_3        = (da + cb) * (da + cb)         in
+    let z_3        = x_1 * ((da - cb) * (da - cb)) in
+    let x_2        = aa * bb                       in
+    let z_2        = e * (aa + (inzp 121665 * e))  in
         ((x_2, z_2), (x_3, z_3)).
 
-lemma eq_op_add_and_double (qx : zp) (nqs : (zp * zp) * (zp * zp)) :
+(* lemma: spec_add_and_double = op_add_and_double *)
+lemma eq_op_add_and_double (qx : zp, nqs : (zp * zp) * (zp * zp)) :
     spec_add_and_double qx nqs = op_add_and_double qx nqs.
 proof.
     rewrite /spec_add_and_double /op_add_and_double.
     auto => />.
 qed.
 
-op op_montgomery_ladder1(init : zp, k : W256.t) =
+(** step 2: montgomery ladder and isolate foldl function and introduce reconstruct tuple * *)
+op op_montgomery_ladder1 (init : zp, k : W256.t) : (zp * zp) * (zp * zp) =
     let nqs0 = ((Zp.one,Zp.zero),(init,Zp.one)) in
     foldl (fun (nqs : (zp * zp) * (zp * zp)) ctr =>
          if spec_ith_bit k ctr
          then spec_swap_tuple (op_add_and_double init (spec_swap_tuple(nqs)))
          else op_add_and_double init nqs) nqs0 (rev (iota_ 0 255)).
+
+op op_montgomery_ladder2_step(k : W256.t, init : zp, nqs : (zp * zp) * (zp * zp), ctr : int) : (zp * zp) * (zp * zp)=
+    if spec_ith_bit k ctr
+    then spec_swap_tuple(op_add_and_double init (spec_swap_tuple(nqs)))
+    else op_add_and_double init nqs.
+
+op op_montgomery_ladder2(init : zp, k : W256.t) : (zp * zp) * (zp * zp) =
+    let nqs0 = reconstruct_triple ((Zp.one,Zp.zero),(init,Zp.one),false) in
+    foldl (op_montgomery_ladder2_step k init) nqs0 (rev (iota_ 0 255)).
 
 (* lemma: spec_montgomery_ladder = op_montgomery_ladder1 *)
 lemma eq_op_montgomery_ladder1 (init : zp) (k : W256.t) :
@@ -91,16 +86,6 @@ proof.
     by move => ?; rewrite /spec_swap_tuple /#.
 qed.
 
-(** step 2: isolate foldl function and introduce reconstruct tuple **)
-op op_montgomery_ladder2_step(k : W256.t, init : zp, nqs : (zp * zp) * (zp * zp), ctr : int) =
-    if spec_ith_bit k ctr
-    then spec_swap_tuple(op_add_and_double init (spec_swap_tuple(nqs)))
-    else op_add_and_double init nqs.
-
-op op_montgomery_ladder2(init : zp, k : W256.t) =
-    let nqs0 = reconstruct_triple ((Zp.one,Zp.zero),(init,Zp.one),false) in
-    foldl (op_montgomery_ladder2_step k init) nqs0 (rev (iota_ 0 255)).
-
 (* lemma: op_montgomery_ladder1 = op_montgomery_ladder2 *)
 lemma eq_op_montgomery_ladder2 (init : zp) (k : W256.t) :
     op_montgomery_ladder1 init k = op_montgomery_ladder2 init k.
@@ -110,21 +95,23 @@ proof.
     by simplify.
 qed.
 
-(** step 3: extend the state to contain an additional bit stating if the state is swapped **)
-op cswap( t : ('a * 'a) * ('a * 'a), b : bool ) =
+
+(** step 3: extend the state to contain an additional bit stating if the state is swapped * *)
+op cswap (t : ('a * 'a) * ('a * 'a), b : bool) : ('a * 'a) * ('a * 'a)  =
     if b
     then spec_swap_tuple t
     else t.
 
-op op_montgomery_ladder3_step(k : W256.t, init : zp, nqs : (zp * zp) * (zp * zp) * bool, ctr : int) =
+op op_montgomery_ladder3_step(k : W256.t, init : zp, nqs : (zp * zp) * (zp * zp) * bool, ctr : int) : (zp * zp) * (zp * zp) * bool =
     let nqs = cswap (select_double_from_triple nqs) (nqs.`3 ^^ (spec_ith_bit k ctr)) in
     let nqs = op_add_and_double init nqs in
     (nqs.`1, nqs.`2, (spec_ith_bit k ctr)).
 
-op op_montgomery_ladder3(init : zp, k : W256.t) =
+op op_montgomery_ladder3(init : zp, k : W256.t) : (zp * zp) * (zp * zp) * bool =
     let nqs0 = ((Zp.one, Zp.zero),(init, Zp.one),false) in
     foldl (op_montgomery_ladder3_step k init) nqs0 (rev (iota_ 0 255)).
 
+(* lemma: op_montgomery_ladder2 = op_reconstruct_triple(op_montgomery_ladder3 ) *)
 lemma eq_op_montgomery_ladder3_reconstruct (init : zp) (k: W256.t) :
     op_montgomery_ladder2 init k = reconstruct_triple (op_montgomery_ladder3 init k).
 proof.
@@ -136,14 +123,14 @@ proof.
     simplify => /#.
 qed.
 
-(* lemma: if the first bit of k is 0, which will be because of spec_decode_scalar_25519, *)
-(*  then op_montgomery_ladder2 = select_double_from_triple op_montgomery_ladder3 *)
-lemma eq_op_montgomery_ladder3 (init : zp) (k: W256.t) :
+(* lemma: if the first bit of k is 0, which will be because of spec_decode_scalar_25519
+   then op_montgomery_ladder2 = select_double_from_triple op_montgomery_ladder3 *)
+lemma eq_op_montgomery_ladder3 (init : zp, k: W256.t) :
     k.[0] = false =>
     op_montgomery_ladder2 init k = select_double_from_triple (op_montgomery_ladder3 init k).
 proof.
     move => hkf.
-    have tbf : (op_montgomery_ladder3 init k).`3 = false. (*third bit false*)
+    have tbf : (op_montgomery_ladder3 init k).`3 = false. (*third bit false *)
     rewrite /op_montgomery_ladder3 /op_montgomery_ladder3_step /select_double_from_triple /cswap /spec_ith_bit /spec_swap_tuple => />.
     rewrite foldl_rev; auto => />; rewrite -iotaredE => />.
     have seqr : select_double_from_triple (op_montgomery_ladder3 init k) = reconstruct_triple (op_montgomery_ladder3 init k).
@@ -152,8 +139,8 @@ proof.
     by apply eq_op_montgomery_ladder3_reconstruct.
 qed.
 
-(** step 4: spec_montgomery_ladder = select_double_from_triple op_montgomery_ladder3 **)
-lemma eq_op_montgomery_ladder123 (init : zp) (k: W256.t) :
+(** step 4: spec_montgomery_ladder = select_double_from_triple op_montgomery_ladder3 * *)
+lemma eq_op_montgomery_ladder123 (init : zp, k: W256.t) :
     k.[0] = false => spec_montgomery_ladder init k = select_double_from_triple (op_montgomery_ladder3 init k).
 proof.
     move => H.
@@ -161,45 +148,46 @@ proof.
     trivial.
 qed.
 
-(** step 5: introduce reordering in encode point **)
+(* step 5: introduce reordering in encode point *)
 (*  - we split invert in 3 parts to make the proof faster *)
-op op_invert_p_p1(z1 : zp) : (zp*zp) =
-    let z2    = ZModpRing.exp z1 2 in
+op op_invert_p_p1 (z1 : zp) : (zp * zp) =
+    let z2    = ZModpRing.exp z1 2     in
     let z8    = ZModpRing.exp z2 (2*2) in
-    let z9    =  z1 * z8 in
-    let z11   = z2  * z9 in
-    let z22   = ZModpRing.exp z11 2 in
-    let z_5_0 = z9  * z22 in
+    let z9    = z1 * z8                in
+    let z11   = z2 * z9                in
+    let z22   = ZModpRing.exp z11 2    in
+    let z_5_0 = z9 * z22               in
         (z_5_0, z11).
 
 op op_invert_p_p2(z_5_0 : zp) : zp =
-    let z_10_5  = ZModpRing.exp z_5_0 (2^5) in
-    let z_10_0  =  z_10_5 * z_5_0 in
+    let z_10_5  = ZModpRing.exp z_5_0 (2^5)   in
+    let z_10_0  =  z_10_5 * z_5_0             in
     let z_20_10 = ZModpRing.exp z_10_0 (2^10) in
-    let z_20_0  = z_20_10 * z_10_0 in
+    let z_20_0  = z_20_10 * z_10_0            in
     let z_40_20 = ZModpRing.exp z_20_0 (2^20) in
-    let z_40_0  = z_40_20 * z_20_0 in
+    let z_40_0  = z_40_20 * z_20_0            in
     let z_50_10 = ZModpRing.exp z_40_0 (2^10) in
     let z_50_0  = z_50_10 * z_10_0 in
         z_50_0.
 
 op op_invert_p_p3(z_50_0 z11 : zp) : zp =
-    let z_100_50  = ZModpRing.exp z_50_0 (2^50) in
-    let z_100_0   =  z_100_50 * z_50_0 in
+    let z_100_50  = ZModpRing.exp z_50_0 (2^50)   in
+    let z_100_0   =  z_100_50 * z_50_0            in
     let z_200_100 = ZModpRing.exp z_100_0 (2^100) in
-    let z_200_0   = z_200_100 * z_100_0 in
-    let z_250_50  = ZModpRing.exp z_200_0 (2^50) in
-    let z_250_0   = z_250_50 * z_50_0 in
-    let z_255_5   = ZModpRing.exp z_250_0 (2^5) in
-    let z_255_21  = z_255_5 *  z11 in
-        z_255_21    .
+    let z_200_0   = z_200_100 * z_100_0           in
+    let z_250_50  = ZModpRing.exp z_200_0 (2^50)  in
+    let z_250_0   = z_250_50 * z_50_0             in
+    let z_255_5   = ZModpRing.exp z_250_0 (2^5)   in
+    let z_255_21  = z_255_5 *  z11                in
+        z_255_21.
 
 op op_invert_p(z1 : zp) : zp =
-    let (z_5_0, z11) = op_invert_p_p1 z1 in
-    let z_50_0       = op_invert_p_p2 z_5_0 in
+    let (z_5_0, z11) = op_invert_p_p1 z1         in
+    let z_50_0       = op_invert_p_p2 z_5_0      in
     let z_255_21     = op_invert_p_p3 z_50_0 z11 in
     z_255_21 axiomatized by op_invert_pE.
 
+(* lemma: invert is the same as z1^(p-2) from fermat's little theorem *)
 lemma eq_op_invert_p (z1: zp) :
     op_invert_p z1 = ZModpRing.exp z1 (p-2).
 proof.
@@ -230,42 +218,45 @@ qed. (* there must be a faster and elegant way of doing this *)
 
 (* now we define invert as one op and prove it equiv to exp z1 (p-2) *)
 op op_invert0(z1 : zp) : zp =
-    let z2        = ZModpRing.exp z1 2 in
-    let z8        = ZModpRing.exp z2 (2*2) in
-    let z9        =  z1 * z8 in
-    let z11       =  z2 * z9 in
-    let z22       = ZModpRing.exp z11 2 in
-    let z_5_0     =   z9 * z22 in
-    let z_10_5    = ZModpRing.exp z_5_0 (2^5) in
-    let z_10_0    =   z_10_5 * z_5_0 in
-    let z_20_10   = ZModpRing.exp z_10_0 (2^10) in
-    let z_20_0    =   z_20_10 * z_10_0 in
-    let z_40_20   = ZModpRing.exp z_20_0 (2^20) in
-    let z_40_0    =   z_40_20 * z_20_0 in
-    let z_50_10   = ZModpRing.exp z_40_0 (2^10) in
-    let z_50_0    =   z_50_10 * z_10_0 in
-    let z_100_50  = ZModpRing.exp z_50_0 (2^50) in
-    let z_100_0   =   z_100_50 * z_50_0 in
+    let z2        = ZModpRing.exp z1 2            in
+    let z8        = ZModpRing.exp z2 (2*2)        in
+    let z9        = z1 * z8                       in
+    let z11       = z2 * z9                       in
+    let z22       = ZModpRing.exp z11 2           in
+    let z_5_0     = z9 * z22                      in
+    let z_10_5    = ZModpRing.exp z_5_0 (2^5)     in
+    let z_10_0    = z_10_5 * z_5_0                in
+    let z_20_10   = ZModpRing.exp z_10_0 (2^10)   in
+    let z_20_0    = z_20_10 * z_10_0              in
+    let z_40_20   = ZModpRing.exp z_20_0 (2^20)   in
+    let z_40_0    = z_40_20 * z_20_0              in
+    let z_50_10   = ZModpRing.exp z_40_0 (2^10)   in
+    let z_50_0    = z_50_10 * z_10_0              in
+    let z_100_50  = ZModpRing.exp z_50_0 (2^50)   in
+    let z_100_0   = z_100_50 * z_50_0             in
     let z_200_100 = ZModpRing.exp z_100_0 (2^100) in
-    let z_200_0   =   z_200_100 * z_100_0 in
-    let z_250_50  = ZModpRing.exp z_200_0 (2^50) in
-    let z_250_0   =  z_250_50 * z_50_0 in
-    let z_255_5   = ZModpRing.exp z_250_0 (2^5) in
-    let z_255_21  =  z_255_5 * z11 in
+    let z_200_0   = z_200_100 * z_100_0           in
+    let z_250_50  = ZModpRing.exp z_200_0 (2^50)  in
+    let z_250_0   = z_250_50 * z_50_0             in
+    let z_255_5   = ZModpRing.exp z_250_0 (2^5)   in
+    let z_255_21  = z_255_5 * z11                 in
         z_255_21 axiomatized by op_invert0E.
 
+(* lemma: op_invert0 = op_invert_p *)
 lemma eq_op_invert0 (z1 : zp) :
     op_invert0 z1 = op_invert_p z1.
 proof.
     rewrite op_invert0E op_invert_pE /op_invert_p_p1 /op_invert_p_p2 /op_invert_p_p3 //.
 qed.
 
+(* lemma: hence, op_invert0 is equal to z1^(p-1) *)
 lemma eq_op_invert0p (z1 : zp) :
     op_invert0 z1 = ZModpRing.exp z1 (p-2).
 proof.
     rewrite eq_op_invert0 eq_op_invert_p //.
 qed.
 
+(* we now need to define various iterated sqaure operations and lemmas *)
 op op_sqr(z : zp) : zp =
     ZModpRing.exp z 2.
 
@@ -281,6 +272,7 @@ op op_it_sqr_x2(e : int, z : zp) : zp =
 op op_it_sqr1_x2(e : int, z : zp) : zp =
     foldl (fun (z' : zp) _ => ZModpRing.exp z' 4) z (iota_ 0 e).
 
+(* lemma: op_it_sqr1 = op_itr_sqr *)
 lemma eq_op_it_sqr1 (e : int, z : zp) :
     0 <= e  =>
     op_it_sqr1 e z = op_it_sqr e z.
@@ -293,6 +285,7 @@ proof.
     rewrite exprS // mulzC //.
 qed.
 
+(* lemma: op_it_sqr1_x2 = op_itr_sqr_x2 *)
 lemma eq_op_it_sqr1_x2 (e : int, z : zp) :
     0 <= e  =>
     op_it_sqr1_x2 e z = op_it_sqr_x2 e z.
@@ -307,6 +300,7 @@ proof.
     rewrite exprS // mulzC //.
 qed.
 
+(* lemma: op_it_sqr = op_itr_sqr_x2 *)
 lemma eq_op_it_sqr_x2_4 (e : int, z : zp) :
     0 <= e  => e %% 2 = 0 =>
     op_it_sqr e z = op_it_sqr_x2 (e%/2) z.
@@ -318,6 +312,7 @@ proof.
     rewrite -exprM => />. smt().
 qed.
 
+(* lemma: op_it_sqr1 = op_itr1_sqr_x2 *)
 lemma eq_op_it_sqr1_x2_4 (e : int, z : zp) :
     0 <= e  => e %% 2 = 0 =>
     op_it_sqr1 e z = op_it_sqr1_x2 (e%/2) z.
@@ -327,6 +322,7 @@ proof.
     apply eq_op_it_sqr_x2_4; trivial.
 qed.
 
+(* lemma: op_it_sqr1 = op_itr_sqr_x2, other perspective *)
 lemma eq_op_it_sqr1_x2_4_twice (e : int, z : zp) :
     0 <= e  => e %% 2 = 0 =>
     op_it_sqr1 (2*e) z = op_it_sqr1_x2 e z.
@@ -338,7 +334,7 @@ proof.
     rewrite -exprM => />.
 qed.
 
-
+(* lemma: op_it_sqr1 with arg 0 *)
 lemma op_it_sqr1_0 (e : int) (z : zp) :
      0 = e => op_it_sqr1 e z = z.
 proof.
@@ -348,6 +344,7 @@ proof.
     rewrite ZModpRing.expr1 //.
 qed.
 
+(* lemma: op_it_sqr1_x2 with arg 0 *)
 lemma op_it_sqr1_x2_0 (e : int) (z : zp) :
      0 = e => op_it_sqr1_x2 e z = z.
 proof.
@@ -357,30 +354,32 @@ proof.
     rewrite ZModpRing.expr1 //.
 qed.
 
+(* lemma: "decomposing" op_it_sqr1 with e-2 *)
 lemma op_it_sqr1_m2_exp4 (e : int) (z : zp) :
      0 <= e - 2 => op_it_sqr1 e z = op_it_sqr1 (e-2) (ZModpRing.exp (ZModpRing.exp z 2) 2).
 proof.
     rewrite expE // /= => ?.
     rewrite !eq_op_it_sqr1. smt(). trivial.
-    rewrite /op_it_sqr (*expE*).
+    rewrite /op_it_sqr (*expE *).
     (* directly rewriting expE takes too long *)
     have ee :  ZModpRing.exp (ZModpRing.exp z 4) (2 ^ (e - 2)) =  ZModpRing.exp z (2^2 * 2 ^ (e - 2)). smt(expE).
     rewrite ee. congr.
     rewrite -exprD_nneg //.
 qed.
 
-
+(* lemma: "decomposing" op_it_sqr1 witg arg e-1 *)
 lemma op_it_sqr1_m2_exp1 (e : int) (z : zp) :
      0 <= e - 1 => op_it_sqr1 e z = op_it_sqr1 (e-1) (ZModpRing.exp z  2).
 proof.
     have ->: ZModpRing.exp z 2 = ZModpRing.exp (ZModpRing.exp z 1) 2. rewrite expE. smt(). trivial.
     rewrite expE // /= => ?.
     rewrite !eq_op_it_sqr1. smt(). smt().
-    rewrite /op_it_sqr (*expE*). rewrite expE. split. smt().
+    rewrite /op_it_sqr (*expE *). rewrite expE. split. smt().
     rewrite expr_ge0 //. congr. have ->: 2 * 2^(e-1) = 2^1 * 2^(e-1). rewrite expr1 //.
     rewrite -exprD_nneg //.
 qed.
 
+(* lemma: "decomposing" op_it_sqr1_x2 with arg e-2 *)
 lemma op_it_sqr1_m2_exp4_x2 (e : int) (z : zp) :
      0 <= e - 2 => op_it_sqr1_x2 e z = op_it_sqr1_x2 (e-2) (ZModpRing.exp (ZModpRing.exp z 4) 4).
 proof.
@@ -393,47 +392,47 @@ proof.
     rewrite -exprD_nneg //.
 qed.
 
+(* lemma: "decomposing" op_it_sqr1_x2 with arg e-1 *)
 lemma op_it_sqr1_m2_exp1_x2 (e : int) (z : zp) :
      0 <= e - 1 => op_it_sqr1_x2 e z = op_it_sqr1_x2 (e-1) (ZModpRing.exp z 4).
 proof.
     have ->: ZModpRing.exp z 4 = ZModpRing.exp (ZModpRing.exp z 1) 4. rewrite expE. smt(). trivial.
     rewrite expE // /= => ?.
     rewrite !eq_op_it_sqr1_x2. smt(). smt().
-    rewrite /op_it_sqr_x2 (*expE*). rewrite expE. split. smt().
+    rewrite /op_it_sqr_x2 (*expE *). rewrite expE. split. smt().
     rewrite expr_ge0 //. congr. have ->: 4 * 4^(e-1) = 4^1 * 4^(e-1). rewrite expr1 //.
     rewrite -exprD_nneg //.
 qed.
 
-
-
 op op_invert1(z1 : zp) : zp =
-    let t0 = op_sqr z1  in        (* z1^2  *)
-    let t1 = op_sqr t0  in        (* z1^4  *)
-    let t1 = op_sqr t1  in        (* z1^8  *)
-    let t1 =  z1 * t1 in        (* z1^9  *)
-    let t0 =  t0 * t1 in        (* z1^11 *)
-    let t2 = op_sqr t0  in        (* z1^22 *)
-    let t1 =  t1 * t2 in        (* z_5_0  *)
-    let t2 = op_sqr t1  in        (* z_10_5 *)
-    let t2 = op_it_sqr 4 t2  in
-    let t1 =  t1 * t2 in        (* z_10_0 *)
-    let t2 = op_it_sqr 10 t1 in   (* z_20_10 *)
-    let t2 =  t1 * t2 in        (* z_20_0 *)
-    let t3 = op_it_sqr 20 t2 in   (* z_40_20 *)
-    let t2 =  t2 * t3 in        (* z_40_0 *)
-    let t2 = op_it_sqr 10 t2 in   (* z_50_10 *)
-    let t1 =  t1 * t2 in        (* z_50_0 *)
-    let t2 = op_it_sqr 50 t1 in   (* z_100_50 *)
-    let t2 =  t1 * t2 in        (* z_100_0 *)
-    let t3 = op_it_sqr 100 t2 in  (* z_200_100 *)
-    let t2 =  t2 * t3 in        (* z_200_0 *)
-    let t2 = op_it_sqr 50 t2 in   (* z_250_50 *)
-    let t1 =  t1 * t2 in        (* z_250_0 *)
-    let t1 = op_it_sqr 4 t1 in    (* z_255_5 *)
-    let t1 = op_sqr t1 in
-    let t1 =  t0 * t1 in
+    let t0 = op_sqr z1        in   (* z1^2  *)
+    let t1 = op_sqr t0        in   (* z1^4  *)
+    let t1 = op_sqr t1        in   (* z1^8  *)
+    let t1 = z1 * t1          in   (* z1^9  *)
+    let t0 = t0 * t1          in   (* z1^11 *)
+    let t2 = op_sqr t0        in   (* z1^22 *)
+    let t1 = t1 * t2          in   (* z_5_0  *)
+    let t2 = op_sqr t1        in   (* z_10_5 *)
+    let t2 = op_it_sqr 4 t2   in
+    let t1 = t1 * t2          in   (* z_10_0 *)
+    let t2 = op_it_sqr 10 t1  in   (* z_20_10 *)
+    let t2 = t1 * t2          in   (* z_20_0 *)
+    let t3 = op_it_sqr 20 t2  in   (* z_40_20 *)
+    let t2 = t2 * t3          in   (* z_40_0 *)
+    let t2 = op_it_sqr 10 t2  in   (* z_50_10 *)
+    let t1 = t1 * t2          in   (* z_50_0 *)
+    let t2 = op_it_sqr 50 t1  in   (* z_100_50 *)
+    let t2 = t1 * t2          in   (* z_100_0 *)
+    let t3 = op_it_sqr 100 t2 in   (* z_200_100 *)
+    let t2 = t2 * t3          in   (* z_200_0 *)
+    let t2 = op_it_sqr 50 t2  in   (* z_250_50 *)
+    let t1 = t1 * t2          in   (* z_250_0 *)
+    let t1 = op_it_sqr 4 t1   in   (* z_255_5 *)
+    let t1 = op_sqr t1        in
+    let t1 = t0 * t1          in
         t1 axiomatized by op_invert1E.
 
+(* lemma: op_invert1 = op_invert0 *)
 lemma eq_op_invert1 (z1: zp) :
     op_invert1 z1 = op_invert0 z1.
 proof.
@@ -441,42 +440,43 @@ proof.
     smt(exprS exprD expE).
 qed.
 
-(** split op_invert2 in 3 parts : jump from op_it_sqr to op_it_sqr1 **)
-
+(* split op_invert2 in 3 parts : jump from op_it_sqr to op_it_sqr1 *)
 op op_invert2(z1 : zp) : zp =
-    let t0 = op_sqr z1  in        (* z1^2  *)
-    let t1 = op_sqr t0  in        (* z1^4  *)
-    let t1 = op_sqr t1  in        (* z1^8  *)
-    let t1 =   z1 * t1 in        (* z1^9  *)
-    let t0 =   t0 * t1 in        (* z1^11 *)
-    let t2 = op_sqr t0  in        (* z1^22 *)
-    let t1 =   t1 * t2 in        (* z_5_0  *)
-    let t2 = op_sqr t1  in        (* z_10_5 *)
-    let t2 = op_it_sqr1 4 t2  in
-    let t1 =   t1 * t2 in        (* z_10_0 *)
-    let t2 = op_it_sqr1 10 t1 in  (* z_20_10 *)
-    let t2 =   t1 * t2 in        (* z_20_0 *)
-    let t3 = op_it_sqr1 20 t2 in  (* z_40_20 *)
-    let t2 =   t2 * t3 in        (* z_40_0 *)
-    let t2 = op_it_sqr1 10 t2 in  (* z_50_10 *)
-    let t1 =   t1 * t2 in        (* z_50_0 *)
-    let t2 = op_it_sqr1 50 t1 in  (* z_100_50 *)
-    let t2 =   t1 * t2 in        (* z_100_0 *)
-    let t3 = op_it_sqr1 100 t2 in (* z_200_100 *)
-    let t2 =   t2 * t3 in        (* z_200_0 *)
-    let t2 = op_it_sqr1 50 t2 in  (* z_250_50 *)
-    let t1 =   t1 * t2 in        (* z_250_0 *)
-    let t1 = op_it_sqr1 4 t1 in   (* z_255_5 *)
-    let t1 = op_sqr t1 in
-    let t1 =   t0 * t1 in
+    let t0 = op_sqr z1         in  (* z1^2  *)
+    let t1 = op_sqr t0         in  (* z1^4  *)
+    let t1 = op_sqr t1         in  (* z1^8  *)
+    let t1 = z1 * t1           in  (* z1^9  *)
+    let t0 = t0 * t1           in  (* z1^11 *)
+    let t2 = op_sqr t0         in  (* z1^22 *)
+    let t1 = t1 * t2           in  (* z_5_0  *)
+    let t2 = op_sqr t1         in  (* z_10_5 *)
+    let t2 = op_it_sqr1 4 t2   in
+    let t1 = t1 * t2           in  (* z_10_0 *)
+    let t2 = op_it_sqr1 10 t1  in  (* z_20_10 *)
+    let t2 = t1 * t2           in  (* z_20_0 *)
+    let t3 = op_it_sqr1 20 t2  in  (* z_40_20 *)
+    let t2 = t2 * t3           in  (* z_40_0 *)
+    let t2 = op_it_sqr1 10 t2  in  (* z_50_10 *)
+    let t1 = t1 * t2           in  (* z_50_0 *)
+    let t2 = op_it_sqr1 50 t1  in  (* z_100_50 *)
+    let t2 = t1 * t2           in  (* z_100_0 *)
+    let t3 = op_it_sqr1 100 t2 in  (* z_200_100 *)
+    let t2 = t2 * t3           in  (* z_200_0 *)
+    let t2 = op_it_sqr1 50 t2  in  (* z_250_50 *)
+    let t1 = t1 * t2           in  (* z_250_0 *)
+    let t1 = op_it_sqr1 4 t1   in  (* z_255_5 *)
+    let t1 = op_sqr t1         in
+    let t1 = t0 * t1           in
         t1 axiomatized by op_invert2E.
 
+(* lemma: op_invert2 = op_invert 1 *)
 lemma eq_op_invert2 (z1: zp) :
     op_invert2 z1 = op_invert1 z1.
 proof.
     rewrite op_invert2E op_invert1E. smt(eq_op_it_sqr1).
 qed.
 
+(* lemma: op_invert2 returns the inverse of its arg *)
 lemma eq_op_invert210p (z1: zp) :
     op_invert2 z1 = ZModpRing.exp z1 (p-2).
 proof.
@@ -486,9 +486,10 @@ qed.
 (* now we define an alternative version of spec_encode_point *)
 op op_encode_point (q: zp * zp) : W256.t =
     let qi = op_invert2 q.`2 in
-    let q =  q.`1 *  qi in
+    let q =  q.`1 * qi       in
         W256.of_int (asint q) axiomatized by op_encode_pointE.
 
+(* lemma: op_encode_point = spec_encode_point *)
 lemma eq_op_encode_point (q: zp * zp) :
     op_encode_point q = spec_encode_point q.
 proof.
@@ -496,13 +497,13 @@ proof.
     rewrite eq_op_invert210p //.
 qed.
 
-(** step 6: spec_scalarmult with updated op_montgomery_ladder3 **)
+(* step 6: spec_scalarmult with updated op_montgomery_ladder3 *)
 
-op op_scalarmult_internal(u: zp) (k:W256.t) : W256.t =
+op op_scalarmult_internal(u: zp, k:W256.t) : W256.t =
     let r = op_montgomery_ladder3 u  k in
         op_encode_point (r.`1) axiomatized by op_scalarmult_internalE.
 
-(* lemma spec_scalarmult = op_scalarmult *)
+(* lemma: spec_scalarmult = op_scalarmult *)
 lemma eq_op_scalarmult_internal (u:zp) (k:W256.t) :
     k.[0] = false => op_scalarmult_internal u k = spec_scalarmult_internal u k.
 proof.
@@ -527,7 +528,7 @@ hint simplify op_scalarmultE.
 op op_scalarmult_base(k:W256.t) : W256.t =
     op_scalarmult (k) (W256.of_int(9%Int)).
 
-(* lemma spec_scalarmult = op_scalarmult *)
+(* lemma: spec_scalarmult = op_scalarmult *)
 lemma eq_op_scalarmult (k:W256.t) (u:W256.t) :
     op_scalarmult k u = spec_scalarmult k u.
 proof.
@@ -543,6 +544,7 @@ proof.
     rewrite ml123 /select_double_from_triple //.
 qed.
 
+(* lemma: spec_ op_scalarmult_base = spec_scalarmult_base *)
 lemma eq_op_scalarmult_base (k:W256.t) :
     op_scalarmult_base k = spec_scalarmult_base k.
 proof.
